src/PermS.v
@@ -1,0 +1,58 @@
+From Heapster Require Import
+     Permissions
+     PermissionsSpred2.
+
+From Coq Require Import
+     Classes.RelationClasses.
+
+Section PermSet.
+  Context {config : Type}.
+
+  Record Perms2 :=
+    {
+      in_Perms2 : forall {spred}, @perm { x | spred x } -> Prop;
+      Perms_upwards_closed1 : forall (spred1 spred2 : config -> Prop)
+                                (Hspred : forall x, spred1 x -> spred2 x)
+                                (p1 : @perm {x | spred1 x}) (p2 : @perm {x | spred2 x}),
+        in_Perms2 p1 ->
+        hlte_perm1 config spred1 spred2 Hspred p1 p2 ->
+        in_Perms2 p2 (* p2 has bigger spred *);
+      (* Perms_upwards_closed2 : forall (spred1 spred2 : config -> Prop) *)
+      (*                           (Hspred : forall x, spred1 x -> spred2 x) *)
+      (*                           (p1 : @perm {x | spred2 x}) (p2 : @perm {x | spred1 x}), *)
+      (*   in_Perms2 p1 -> *)
+      (*   hlte_perm2 config spred1 spred2 Hspred p1 p2 -> *)
+      (*   in_Perms2 p2 (* p2 has smaller spred *) *)
+    }.
+  Notation "p ∈2 P" := (in_Perms2 P p) (at level 60).
+
+
+  Definition lte_Perms2 (P Q : Perms2) : Prop :=
+    forall spred (p : @perm {x | spred x}), p ∈2 Q -> p ∈2 P.
+  Notation "P ⊑2 Q" := (lte_Perms2 P Q) (at level 60).
+
+  Program Definition top_Perms2 : Perms2 :=
+    {|
+      in_Perms2 := fun _ _ => False
+    |}.
+  Program Definition bottom_Perms2 : Perms2 :=
+    {|
+      in_Perms2 := fun _ _ => True
+    |}.
+
+  Program Definition sep_conj_Perms2 (P Q : Perms2) : Perms2 :=
+    {|
+      in_Perms2 := fun spred r =>
+                     exists spred' Hspred (p q : @perm {x | spred' x}),
+                       in_Perms2 P p /\
+                         in_Perms2 Q q /\
+                         hlte_perm1 config spred' spred Hspred (p ** q) r
+    |}.
+  Next Obligation.
+    rename H into spred', H1 into Hspred', H2 into p, H3 into q.
+    exists spred'. eexists. Unshelve.
+    2: { intros. auto. }
+    exists p, q. split; [| split]; auto. eapply hlte_perm1_transitive; eauto.
+  Qed.
+
+End PermSet.
