src/SepStepSpred2.v
@@ -1,0 +1,109 @@
+(* begin hide *)
+From Heapster Require Import
+     Permissions
+     PermissionsSpred2.
+
+From Coq Require Import
+     Classes.RelationClasses.
+(* end hide *)
+
+Section step.
+  Context (config : Type).
+  Context (spred spred' : config -> Prop).
+  (* Context {spred2 spred2' : specConfig -> Prop}. *)
+  Context (Hspred : forall x, spred x -> spred' x).
+  (* Context (Hspred2 : forall x, spred2 x -> spred2' x). *)
+  (* TODO: change to 1 spred *)
+
+  (** * Preserves separability *)
+  Definition sep_step
+             (p : @perm ({x | spred' x}))
+             (q : @perm ({x | spred x})) : Prop :=
+    forall r, p ⊥ r -> q ⊥ (restrict _ _ _ Hspred r).
+End step.
+
+Global Instance sep_step_refl config spred : Reflexive (sep_step config spred spred (fun x H => H)).
+Proof.
+  repeat intro; auto. rewrite restrict_same. auto.
+Qed.
+
+(* Global Instance sep_step_trans : Transitive sep_step. *)
+(* Proof. *)
+(*   repeat intro. auto. *)
+(* Qed. *)
+
+Lemma sep_step_lte config (spred1 spred2 : config -> Prop) Hspred :
+  forall p p' q, p <= p' ->
+            sep_step config spred1 spred2 Hspred p q ->
+            sep_step config spred1 spred2 Hspred p' q.
+Proof.
+  repeat intro. apply H0. symmetry. symmetry in H1. eapply separate_antimonotone; eauto.
+Qed.
+
+(* Lemma sep_step_lte' : forall p q, q <= p -> sep_step p q. *)
+(* Proof. *)
+(*   repeat intro. symmetry. eapply separate_antimonotone; eauto. symmetry; auto. *)
+(* Qed. *)
+
+(* Program Definition sym_guar_perm (p : @perm config) : perm := *)
+(*   {| *)
+(*     pre x := False; *)
+(*     rely := guar p; *)
+(*     guar := rely p; *)
+(*   |}. *)
+(* Lemma separate_self_sym : forall p, p ⊥ sym_guar_perm p. *)
+(* Proof. *)
+(*   intros. split; intros; auto. *)
+(* Qed. *)
+
+(* Lemma sep_step_rely : forall p q x y, sep_step p q -> *)
+(*                                  rely p x y -> *)
+(*                                  rely q x y. *)
+(* Proof. *)
+(*   intros. specialize (H (sym_guar_perm p) (separate_self_sym _)). *)
+(*   apply H; auto. *)
+(* Qed. *)
+
+(* Lemma sep_step_guar : forall p q x y, sep_step p q -> *)
+(*                                  guar q x y -> *)
+(*                                  guar p x y. *)
+(* Proof. *)
+(*   intros. specialize (H (sym_guar_perm p) (separate_self_sym _)). *)
+(*   apply H; auto. *)
+(* Qed. *)
+
+(* Lemma sep_step_rg : forall p q, *)
+(*     (forall x y, guar q x y -> guar p x y) -> *)
+(*     (forall x y, rely p x y -> rely q x y) -> *)
+(*     sep_step p q. *)
+(* Proof. *)
+(*   repeat intro. split; intros. *)
+(*   - apply H0. apply H1. auto. *)
+(*   - apply H1. apply H. auto. *)
+(* Qed. *)
+
+(* Lemma sep_step_iff : forall p q, *)
+(*     sep_step p q <-> (forall x y, rely p x y -> rely q x y) /\ (forall x y, guar q x y -> guar p x y). *)
+(* Proof. *)
+(*   split; [split; intros; [eapply sep_step_rely | eapply sep_step_guar] | *)
+(*            intros []; apply sep_step_rg]; eauto. *)
+(* Qed. *)
+
+Lemma sep_step_sep_conj_l config spred1 spred2 Hspred :
+  forall p1 p2 q, p1 ⊥ q ->
+             sep_step config spred1 spred2 Hspred p1 p2 ->
+             sep_step config spred1 spred2 Hspred (p1 ** q) (p2 ** q).
+Proof.
+  intros p1 p2 q ? ?.
+  repeat intro; auto. symmetry in H1. symmetry. apply separate_sep_conj_perm; symmetry; auto.
+  - apply H0. symmetry. eapply separate_sep_conj_perm_l; eauto.
+  - symmetry. eapply separate_sep_conj_perm_r; eauto.
+Qed.
+Lemma sep_step_sep_conj_r : forall p1 p2 q, p1 ⊥ q -> sep_step p1 p2 -> sep_step (q ** p1) (q ** p2).
+Proof.
+  intros p1 p2 q ? ?.
+  repeat intro; auto. symmetry in H1. symmetry. apply separate_sep_conj_perm; symmetry; auto.
+  - symmetry. eapply separate_sep_conj_perm_l; eauto.
+  - apply H0. symmetry. eapply separate_sep_conj_perm_r; eauto.
+  - symmetry. auto.
+Qed.
